proof/invariant-abstract/RISCV64/ArchInterrupt_AI.thy
@@ -45,7 +45,7 @@ lemma decode_irq_control_valid [Interrupt_AI_assms]:
                  split del: if_split cong: if_cong)
   apply (wpsimp wp: ensure_empty_stronger simp: cte_wp_at_eq_simp arch_irq_control_inv_valid_def
          | wp (once) hoare_drop_imps)+
-  apply (clarsimp simp: linorder_not_less word_le_nat_alt unat_ucast maxIRQ_def)
+  apply (clarsimp simp: linorder_not_less word_le_nat_alt unat_ucast maxIRQ_def Kernel_Config.maxIRQ_def)
   apply (cases caps; clarsimp simp: cte_wp_at_eq_simp)
   apply (intro conjI impI; clarsimp)
   apply (drule ucast_ucast_mask_eq)
