proof/refine/RISCV64/ArchInterrupt_R.thy
@@ -17,7 +17,7 @@ named_theorems Interrupt_R_assms
 
 lemma maxIRQ_H_ucast_toEnum_eq_irq[Interrupt_R_assms]:
   "x \<le> ucast maxIRQ \<Longrightarrow> toEnum (unat x) = (ucast x :: irq)" for x::machine_word
-  by (simp add: word_le_nat_alt maxIRQ_def)
+  by (simp add: word_le_nat_alt maxIRQ_def Kernel_Config.maxIRQ_def)
 
 lemma arch_valid_irq_le_maxIRQ[Interrupt_R_assms]:
   "arch_valid_irq irq \<Longrightarrow> irq \<le> maxIRQ"
@@ -67,7 +67,7 @@ lemma checkIRQ_irq_valid[Interrupt_R_assms]:
   apply (clarsimp simp: unlessE_def split del: if_split)
   apply (wpsimp simp: maxIRQ_H_ucast_toEnum_eq_irq)
   apply (simp add: not_less word_le_nat_alt unat_ucast_upcast is_up unat_ucast_unat_id
-                   maxIRQ_def irqInvalid_def
+                   maxIRQ_def Kernel_Config.maxIRQ_def irqInvalid_def
               flip: word_unat.Rep_inject)
   done
 
@@ -127,7 +127,7 @@ lemma arch_decode_irq_control_valid'[Interrupt_R_assms, wp]:
           | wpc
           | wp (once) hoare_drop_imps)+
   apply (clarsimp simp: invs_valid_objs' not_less maxIRQ_H_ucast_toEnum_eq_irq word_le_nat_alt
-                        unat_ucast_upcast is_up unat_ucast_unat_id maxIRQ_def
+                        unat_ucast_upcast is_up unat_ucast_unat_id maxIRQ_def Kernel_Config.maxIRQ_def
                   simp flip: word_unat.Rep_inject)
   done
 
